

# MATH 7337: Harmonic Analysis

Frank Qiang  
Instructor: Christopher Heil

Georgia Institute of Technology  
Fall 2025

# Contents

<b>1</b>	<b>Aug. 19 — The Fourier Transform</b>	<b>2</b>
1.1	The Fourier Transform on $L^1(\mathbb{R})$ . . . . .	2
1.2	Motivation for the Fourier Transform . . . . .	3
<b>2</b>	<b>Aug. 21 — The Riemann-Lebesgue Lemma</b>	<b>4</b>
2.1	Properties of the Fourier Transform . . . . .	4
2.2	The Riemann-Lebesgue Lemma . . . . .	4
2.3	Position and Momentum Operators . . . . .	6
2.4	The HRT Conjecture . . . . .	6
<b>3</b>	<b>Aug. 3 — Convolution</b>	<b>7</b>
3.1	Convolution . . . . .	7
3.2	Properties of Convolution . . . . .	7
3.3	Young's Inequality . . . . .	9
3.4	The Dirac Delta . . . . .	10
<b>4</b>	<b>Aug. 28 — Convolution, Part 2</b>	<b>11</b>
<b>5</b>	<b>Sept. 2 — Smoothness and Decay</b>	<b>12</b>
5.1	Smoothness and Decay . . . . .	12
5.2	Absolute Continuity . . . . .	13
5.3	Smoothness and Decay, Continued . . . . .	14
5.4	Approximate Identities . . . . .	14
<b>6</b>	<b>Sept. 4 — Approximate Identities</b>	<b>16</b>
6.1	Properties of Approximate Identities . . . . .	16
6.2	Density Results and Smooth Urysohn Lemma . . . . .	18
<b>7</b>	<b>Sept. 18 —</b>	<b>19</b>
<b>8</b>	<b>Sept. 23 —</b>	<b>20</b>
<b>9</b>	<b>Sept. 25 — Kernels and Schwartz Space</b>	<b>21</b>
9.1	More Kernels . . . . .	21
9.2	Schwartz Space . . . . .	22

# Lecture 1

## Aug. 19 — The Fourier Transform

### 1.1 The Fourier Transform on $L^1(\mathbb{R})$

All integrals will be taken over  $\mathbb{R}$  unless otherwise specified.

**Definition 1.1.** The *Fourier transform* of  $f \in L^1(\mathbb{R})$  is

$$\widehat{f}(\xi) = \int f(x) e^{-2\pi i \xi x} dx, \quad \xi \in \mathbb{R}.$$

**Remark.** Note that by the triangle inequality,

$$|\widehat{f}(\xi)| \leq \int |f(x) e^{-2\pi i \xi x}| dx = \int |f(x)| dx = \|f\|_1 < \infty,$$

so  $\widehat{f}(\xi)$  exists for all  $\xi \in \mathbb{R}$  (in fact,  $\widehat{f}$  is continuous).

**Remark.** The Fourier transform is an operator  $\mathcal{F} : L^1(\mathbb{R}) \rightarrow L^\infty(\mathbb{R})$  as  $\|\widehat{f}\|_\infty = \text{ess sup}_{\xi \in \mathbb{R}} |\widehat{f}(\xi)| \leq \|f\|_1$ . This is linear in  $f$ . The *operator norm* of  $\mathcal{F}$  is

$$\|\mathcal{F}\| = \|\mathcal{F}\|_{L^1 \rightarrow L^\infty} = \sup_{\|f\|_1=1} \|\widehat{f}\|_\infty \leq \sup_{\|f\|_1=1} \|f\|_1 = 1,$$

so  $\mathcal{F}$  is a bounded linear operator. However,  $\mathcal{F}$  is not isometric (norm-preserving) in general.

**Remark.** Observe that

$$\widehat{f}(0) = \int f(x) e^{-2\pi i \cdot 0 \cdot x} dx = \int f(x) dx.$$

So if  $f \geq 0$  and we normalize  $f$  so that  $\widehat{f}(0) = 1$ , then we have

$$|\widehat{f}(\xi)| \leq \int f(x) dx = \widehat{f}(0),$$

and so  $\|\widehat{f}\|_\infty = \text{ess sup}_{\xi \in \mathbb{R}} |\widehat{f}(\xi)| \leq 1$ . This is one particular case where  $\mathcal{F}$  does preserve the norm.

**Definition 1.2.** For  $r \neq 0$ , *dilation* of  $f$  by  $r$  is  $f_r(x) = r f(rx)$ . Note that  $\|f_r\|_1 = \|f\|_1$ .

**Example 1.2.1.** The *Dirichlet function* is  $d(\xi) = \sin(\xi)/\pi\xi \in C_0(\mathbb{R})$ .<sup>1</sup> Note that  $d \notin L^1(\mathbb{R})$ . We can also define the *sinc* function as  $\text{sinc } \xi = \sin(\pi\xi)/(\pi\xi) = d\pi(x)$ .

---

<sup>1</sup>Recall that  $C_0(\mathbb{R})$  is the space of continuous functions  $f : \mathbb{R} \rightarrow \mathbb{C}$  such that  $\lim_{x \rightarrow \pm\infty} f(x) = 0$ .

However,  $d$  is the Fourier transform of a function in  $L^1(\mathbb{R})$ . Consider the

$$\chi_{-[T,T]}(x) = \begin{cases} 1 & \text{if } |x| \leq T, \\ 0 & |x| > T. \end{cases}$$

Note that  $\chi_{-[T,T]} \in L^1(\mathbb{R})$ . Then we have

$$\widehat{\chi}_{-[T,T]}(\xi) = \int_{-T}^T e^{-2\pi i \xi x} dx = \frac{e^{-2\pi i \xi x}}{-2\pi i \xi} \Big|_{-T}^T = \frac{\sin(2\pi T \xi)}{\pi \xi} = d_{2\pi T}(\xi),$$

so we see that  $\widehat{\chi}_{-[T,T]} \in C_0(\mathbb{R}) \subsetneq L^\infty(\mathbb{R})$ .

**Remark.** We will see in general that  $\mathcal{F} : L^1(\mathbb{R}) \rightarrow C_0(\mathbb{R})$ , this is the Riemann-Lebesgue lemma. The image of  $\mathcal{F}$  is a proper dense subspace of  $C_0(\mathbb{R})$ , which implies that  $\mathcal{F}^{-1}$  must be unbounded as a linear operator by Banach space theory.

**Proposition 1.1.** *If  $f \in L^1(\mathbb{R})$ , then  $\widehat{f}$  is uniformly continuous on  $\mathbb{R}$ , i.e.*

$$\|\widehat{f} - T_\eta \widehat{f}\|_\infty = \sup_{\xi \in \mathbb{R}} |\widehat{f}(\xi) - \widehat{f}(\xi - \eta)| \xrightarrow{\eta \rightarrow 0} 0,$$

where  $T_\eta \widehat{f}(\xi) = \widehat{f}(\xi - \eta)$ .

*Proof.* We can write the difference as

$$|\widehat{f}(\xi) - \widehat{f}(\xi - \eta)| = \left| \int f(x)(e^{-2\pi i \xi x} - e^{-2\pi i (\xi - \eta)x}) dx \right| \leq \int |f(x)| |e^{-2\pi i \xi x} - e^{-2\pi i (\xi - \eta)x}| dx.$$

Note that  $f \in L^1(\mathbb{R})$  and  $|e^{-2\pi i \xi x} - e^{-2\pi i (\xi - \eta)x}| = |1 - e^{2\pi i \eta x}| \rightarrow 0$  as  $\eta \rightarrow 0$  independent of  $\xi$ , so the statement follows from the dominated convergence theorem (the integrand is dominated by  $2|f|$ ).  $\square$

## 1.2 Motivation for the Fourier Transform

**Remark.** We will define the *inverse Fourier transform* of  $f \in L^1(\mathbb{R})$  as

$$\check{f}(x) = \int f(\xi) e^{2\pi i \xi x} d\xi.$$

Note that  $\check{f}(\xi) = \widehat{f}(-\xi)$ . With enough assumptions, this is an inverse to the Fourier transform.

**Proposition 1.2** (Fourier inversion formula). *If  $f, \widehat{f} \in L^1(\mathbb{R})$ , then*

$$f(x) = (\widehat{f})^\vee(x) = \int \widehat{f}(\xi) e^{2\pi i \xi x} d\xi.$$

**Remark.** Note that  $e_\xi(x) = e^{2\pi i \xi x} = \cos 2\pi \xi x + i \sin 2\pi \xi x$  and  $e_\xi : \mathbb{R} \rightarrow S^1 = \{z \in \mathbb{C} : |z| = 1\}$ . We have  $e_\xi(x + y) = e_\xi(x)e_\xi(y)$ , so  $e_\xi$  is a homomorphism, and it is also continuous. Thus  $e_\xi$  is a *character* on  $\mathbb{R}$  (in fact, every character on  $\mathbb{R}$  is of the form  $e_\xi$  for some  $\xi$ ). One can use this idea to define Fourier transforms in much more general settings.

**Remark.** The Fourier transform decomposes a function  $f$  into the pure harmonics  $e_\xi$ , and the inversion formula says that we can recover  $f$  as a “sum” of these pure harmonics.

# Lecture 2

## Aug. 21 — The Riemann-Lebesgue Lemma

### 2.1 Properties of the Fourier Transform

**Definition 2.1.** Define the following operators:

1. *Translation:*  $T_a f(x) = f(x - a)$  for  $a \in \mathbb{R}$ ;
2. *Modulation:*  $M_b f(x) = e^{2\pi i b x} f(x)$  for  $b \in \mathbb{R}$ ;
3. *Dilation:*  $f_\lambda(x) = \lambda f(\lambda x)$  for  $\lambda > 0$ ;
4. *Involution:*  $\tilde{f}(x) = \overline{f(-x)}$ .

**Remark.** Translation and modulation are isometries on  $L^p(\mathbb{R})$  for any  $p$ . Dilation as defined above is  $L^1$ -normalized, so it is only an isometry on  $L^1(\mathbb{R})$ .

**Exercise 2.1.** If  $f \in L^1(\mathbb{R})$ , then

1.  $(T_a f)^\wedge(\xi) = (M_{-a} \hat{f})(\xi) = e^{-2\pi i \xi a} \hat{f}(\xi)$ ;
2.  $(M_b f)^\wedge(\xi) = (T_b \hat{f})(\xi) = \hat{f}(\xi - b)$ ;
3.  $(f_\lambda)^\wedge(\xi) = \lambda (f_{1/\lambda})^\wedge(\xi) = \hat{f}(\xi/\lambda)$ ;<sup>1</sup>
4.  $(\bar{f})^\wedge(\xi) = (\hat{f})^\sim(\xi) = \overline{\hat{f}(-\xi)}$ ;
5.  $(\tilde{f})^\wedge(\xi) = \overline{\hat{f}(\xi)}$ .

### 2.2 The Riemann-Lebesgue Lemma

**Definition 2.2.** Let  $C_c(\mathbb{R})$  be the space of continuous functions with compact support. For a continuous function, the *support* of  $f$ , denoted  $\text{supp}(f) = \overline{\{x \in \mathbb{R} : f(x) \neq 0\}}$ . So for a continuous function  $f$ ,  $\text{supp}(f)$  is compact if and only if  $f = 0$  outside some finite interval.

**Theorem 2.1.**  $C_c(\mathbb{R})$  is dense in  $L^p(\mathbb{R})$  for  $1 \leq p < \infty$ . In other words,

1. the closure of  $C_c(\mathbb{R})$  in  $L^p(\mathbb{R})$  is all of  $L^p(\mathbb{R})$ ;
2. for any  $f \in L^p(\mathbb{R})$  and  $\epsilon > 0$ , there exists  $g \in C_c(\mathbb{R})$  such that  $\|f - g\|_p < \epsilon$ ;
3. if  $f \in L^p(\mathbb{R})$ , then there exists  $g_n \in C_c(\mathbb{R})$  such that  $g_n \rightarrow f$  in  $L^p$ -norm, i.e.  $\|g_n - f\|_p \rightarrow 0$ .

---

<sup>1</sup>Note that the result is an  $L^\infty$ -normalized dilation.

For  $p = \infty$ ,  $C_c(\mathbb{R})$  is dense in  $C_0(\mathbb{R})$  with respect to the  $L^\infty$ -norm (this is the same as the uniform norm for continuous functions).

*Proof.* We sketch the proof. First approximate  $f \in L^p(\mathbb{R})$  by a simple function (one that takes only finitely many distinct values)  $\phi = \sum_{k=1}^N c_k \chi_{E_k}$ , e.g. by rounding down to the nearest integer multiple of  $2^{-n}$ . Then use Urysohn's lemma to approximate  $\chi_{E_k}$  by a continuous function.  $\square$

**Exercise 2.2.** Fix  $1 \leq p < \infty$ . Prove that if  $f \in L^p(\mathbb{R})$ , then  $\lim_{a \rightarrow 0} \|f - T_a f\|_p = 0$ . We say that translation is *strongly continuous* on  $L^p(\mathbb{R})$ . For  $p = \infty$ , use  $C_0(\mathbb{R})$  and the uniform norm instead.

**Lemma 2.1** (Riemann-Lebesgue lemma). *If  $f \in L^1(\mathbb{R})$ , then  $\widehat{f} \in C_0(\mathbb{R})$ ,*

*Proof.* We have already seen that  $\widehat{f}$  is continuous. So it suffices to show decay at  $\infty$ . Write

$$\widehat{f}(\xi) = - \int f(x) e^{-2\pi i \xi x} e^{-2\pi i \xi (1/2\xi)} dx = - \int_{-\infty}^{\infty} f(x) e^{-2\pi i \xi (x+1/2\xi)} dx.$$

Now make the change of variables  $x \mapsto x - 1/2\xi$ , so we get

$$\widehat{f}(\xi) = - \int_{-\infty}^{\infty} f\left(x - \frac{1}{2\xi}\right) e^{-2\pi i \xi x} dx = - \int T_{1/2\xi} f(x) e^{-2\pi i \xi x} dx.$$

Taking an average with the usual expression for  $\widehat{f}(\xi)$ , we have

$$\widehat{f}(\xi) = \frac{1}{2} \int (f(x) - T_{1/2\xi} f(x)) e^{-2\pi i \xi x} dx.$$

Taking absolute values, we obtain

$$|\widehat{f}(\xi)| \leq \frac{1}{2} \int |f(x) - T_{1/2\xi} f(x)| dx = \frac{1}{2} \|f - T_{1/2\xi} f\|_1 \xrightarrow{\xi \rightarrow \pm\infty} 0$$

by the strong continuity of translation on  $L^1(\mathbb{R})$ .  $\square$

**Exercise 2.3.** The following is an alternative proof of the Riemann-Lebesgue lemma. Recall that we have  $\widehat{\chi}_{-T,T} = d_{2\pi T} \in C_0(\mathbb{R})$ . By taking translations and dilations, we see that  $\widehat{\chi}_{[a,b]} \in C_0(\mathbb{R})$ . Consider *really simple functions*  $\phi = \sum_{k=1}^N c_k \chi_{[a_k, b_k]}$ , and by linearity we can write

$$\widehat{\phi} = \sum_{k=1}^N c_k \widehat{\chi}_{[a_k, b_k]} \in C_0(\mathbb{R}).$$

Note that really simple functions are also dense in  $L^p(\mathbb{R})$  for  $1 \leq p < \infty$ . So if  $f \in L^1(\mathbb{R})$ , there exist really simple  $\phi_n \rightarrow f$  in  $L^1$ -norm. On the Fourier side, we have

$$\|\widehat{f} - \widehat{\phi}_n\|_\infty \leq \|f - \phi_n\|_1 \rightarrow 0.$$

Since  $\phi_n \rightarrow f$  uniformly and  $C_0(\mathbb{R})$  is a Banach space, we conclude  $\widehat{f} \in C_0(\mathbb{R})$ . Fill in the details.

## 2.3 Position and Momentum Operators

**Definition 2.3.** The *position operator*  $P : L^1(\mathbb{R}) \rightarrow L^1(\mathbb{R})$  is given by  $Pf(x) = xf(x)$ . Note that  $P$  is unbounded on  $L^1(\mathbb{R})$  (in fact,  $P$  is not defined on all of  $L^1(\mathbb{R})$ ). Restrict  $P$  to the domain

$$D_P = \{f \in L^1(\mathbb{R}) : xf(x) \in L^1(\mathbb{R})\},$$

which is dense in  $L^1(\mathbb{R})$ . Note that  $D_P$  cannot be bounded as it does not admit an extension to  $L^1(\mathbb{R})$ .

**Exercise 2.4.** Show that  $\sup_{\|f\|_1=1, f \in D_P} \|Pf\|_1 = \infty$ .

**Definition 2.4.** The *momentum operator*  $M : L^1(\mathbb{R}) \rightarrow L^1(\mathbb{R})$  is given by  $Mf = f'/2\pi i$ . Similarly,  $M$  is unbounded and defined only on a dense subset of  $L^1(\mathbb{R})$ .

**Remark.** We have the relation  $(Mf)^\wedge(\xi) = \xi P\hat{f}(\xi)$ , whenever the statement makes sense.

## 2.4 The HRT Conjecture

**Conjecture 2.1** (HRT conjecture). Assume  $g$  is not zero a.e.,  $a_k, b_k$  are distinct, and consider finite linear combinations of translations and modulations of  $g \in L^2(\mathbb{R})$  of the following form:

$$\sum_{k=1}^N c_k e^{2\pi i b_k x} g(x - a_k). \quad (*)$$

If  $(*) = 0$ , then must it be that  $c_1 = \dots = c_N = 0$ ? In other words, are these linearly independent?

**Remark.** Consider the special case  $b_k = 0$  for every  $k$ , so  $\sum c_k T_{a_k} g = \sum c_k g(x - a_k) = 0$  a.e. Then

$$\left( \sum c_k T_{a_k} g \right)^\wedge = \sum c_k M_{-a_k} \hat{g} = \left( \sum_{k=1}^N c_k e^{-2\pi i a_k \xi} \right) \hat{g}(\xi) = 0.$$

Since  $\hat{g}$  is not zero a.e., we must have  $\sum_{k=1}^N c_k e^{-2\pi i a_k \xi} = 0$ , which implies  $c_k = 0$  for all  $k$ . In particular, this means that translations alone are linearly independent (the same is true for modulations alone).

**Remark.** The general case of the HRT conjecture is still open. Note that after taking a Fourier transform, we end up with the same problem, just for  $\hat{g}$  instead of  $g$ .

# Lecture 3

## Aug. 3 — Convolution

### 3.1 Convolution

**Definition 3.1.** If  $f, g$  are measurable on  $\mathbb{R}$ , their *convolution* is (formally)

$$(f * g)(x) = \int_{-\infty}^{\infty} f(y)g(x-y) dy.$$

**Remark.** When it exists, we have

$$(f * g)(x) = \int_{-\infty}^{\infty} f(y)g(x-y) dy = \int_{-\infty}^{\infty} f(x-y)g(y) dy = (g * f)(x)$$

by the change of variables  $y \mapsto x - y$ . So  $f * g = g * f$ , if it exists. Similarly,  $f * (g * h) = (f * g) * h$  if each of these convolutions exist.

**Remark.** If we take  $g_T = \chi_{-T,T}/2T$  (note that  $\|g_T\|_1 = 1$ ), then

$$(f * g_T)(x) = \int_{-\infty}^{\infty} f(y)g_T(x-y) dy = \frac{1}{2T} \int_{x-T}^{x+T} f(y) dy = \text{Avg}_{[-T,T]} f(x),$$

so we can see convolution as a averaging or smoothing operation (also known as *mollification*).

**Remark.** We would like to show  $f, g \in L^1(\mathbb{R})$  implies  $f * g \in L^1(\mathbb{R})$ . Note that  $(f * g)^\wedge = \widehat{f\widehat{g}} \in C_0(\mathbb{R})$ , since  $C_0(\mathbb{R})$  is closed under multiplication, even though  $L^1(\mathbb{R})$  is not.

**Remark.** The *Lebesgue differentiation theorem* says that if  $f \in L^1_{\text{loc}}(\mathbb{R})$ , then  $(f * g_T)(x) \rightarrow f(x)$  a.e.

### 3.2 Properties of Convolution

**Remark.** Use the notation

$$\langle f, g \rangle = \int_{-\infty}^{\infty} f(x)\overline{g(x)} dx,$$

whenever this integral exists. Then *Hölder's inequality* says that if  $1/p + 1/p' = 1$  with  $1 \leq p \leq \infty$  and  $f \in L^p(\mathbb{R})$ ,  $g \in L^{p'}(\mathbb{R})$ , then  $fg \in L^1(\mathbb{R})$  and we have

$$|\langle f, g \rangle| \leq \int |f(x)||g(x)| dx \leq \|f\|_p \|g\|_{p'}.$$



**Theorem 3.1.** For  $1 \leq p \leq \infty$ , if  $f \in L^p(\mathbb{R})$  and  $g \in L^1(\mathbb{R})$ , then  $f * g \in L^\infty(\mathbb{R})$ .

*Proof.* By Hölder's inequality, we can write

$$\int |f(y)g(x-y)| dy \leq \|f\|_p \|g(x)\|_{p'} < \infty,$$

so  $(f * g)(x)$  exists for every  $x \in \mathbb{R}$ . □

**Exercise 3.1.** Show that  $f * g \in C_b(\mathbb{R}) = \{h : \mathbb{R} \rightarrow \mathbb{C} : h \text{ is continuous and bounded}\}$ .

**Remark.** Denote  $g^*(y) = \overline{g(-y)}$ . Then we have

$$(f * g)(x) = \int f(y)g(x-y) dy = \int f(y)\overline{g^*(y-x)} dy = \langle f, T_x g^* \rangle.$$

**Theorem 3.2.** Let  $f, g \in L^1(\mathbb{R})$ . Then

1.  $f(y)g(x-y)$  is measurable and integrable on  $\mathbb{R}^2$ ;
2. for a.e.  $x \in \mathbb{R}$ ,  $f(y)g(x-y)$  is measurable and integrable on  $\mathbb{R}$  as a function of  $y$ ;
3.  $f * g \in L^1(\mathbb{R})$  and  $\|f * g\|_1 \leq \|f\|_1 \|g\|_1$ , i.e. convolution is submultiplicative on  $L^1(\mathbb{R})$ ;
4.  $(f * g)^\wedge(\xi) = \widehat{f}(\xi)\widehat{g}(\xi)$  for every  $\xi \in \mathbb{R}$ .

*Proof.* (1) Let  $h(x, y) = f(y)g(x-y)$ . Then we have

$$\{h > a\} = h^{-1}((a, \infty)) = \{(x, y) : f(y)g(x-y) > a\} = \{f > a\} \times \mathbb{R},$$

which is measurable in  $\mathbb{R}^2$  since  $\{f > a\}$  and  $\mathbb{R}$  are measurable in  $\mathbb{R}$ . Similarly,  $g(y)$  is measurable on  $\mathbb{R}^2$ , so  $F(x, y) = f(y)g(x-y)$  is measurable on  $\mathbb{R}^2$ . Now make a linear change of variables  $T(x, y) = (y, x-y)$ , so  $H = F \circ T = f(y)g(x-y)$  is measurable (note that linear maps preserve measurability).

Now we can integrate by Tonelli's theorem and see that

$$\begin{aligned} \iint |f(y)g(x-y)| dx dy &= \int |f(y)| \left( \int |g(x-y)| dx \right) dy = \int |f(y)| \left( \int |g(z)| dz \right) dy \\ &= \int |f(y)| \|g\|_1 dy = \|f\|_1 \|g\|_1 < \infty, \end{aligned}$$

hence  $f(y)g(x-y)$  is integrable on  $\mathbb{R}^2$ .

(2) This follows by Fubini's theorem since  $f(y)g(x-y)$  is integrable.

(3) By (2),  $(f * g)(x)$  exists for a.e.  $x$ , and

$$\int |(f * g)(x)| dx = \int \left| \int f(y)g(x-y) dy \right| dx \leq \iint |f(y)g(x-y)| dy dx \leq \|f\|_1 \|g\|_1,$$

which is the desired inequality.

(4) Justify the following calculation as an exercise via Fubini/Tonelli's theorem:

$$\begin{aligned}(f * g)^\wedge(\xi) &= \int (f * g)(x) e^{-2\pi i \xi x} dx = \int \left( \int f(y) g(x - y) dy \right) e^{-2\pi i \xi x} dx \\ &= \iint f(y) e^{-2\pi i \xi y} g(x - y) e^{-2\pi i \xi (x - y)} dy dx.\end{aligned}$$

By Fubini's theorem, we can exchange orders and write

$$\begin{aligned}(f * g)^\wedge(\xi) &= \int f(y) e^{-2\pi i \xi y} \left( \int g(x - y) e^{-2\pi i \xi (x - y)} dx \right) dy \\ &= \int f(y) e^{-2\pi i \xi y} \left( \int g(z) e^{-2\pi i \xi z} dz \right) dy = \widehat{f}(\xi) \widehat{g}(\xi),\end{aligned}$$

which is the desired equality. □

**Corollary 3.2.1.**  $L^1(\mathbb{R})$  is closed under convolution.

**Definition 3.2.** An *algebra* is a vector space  $A$  with a product such that

- (a)  $(fg)h = f(gh)$ ,
- (b)  $f(g + h) = fg + fh$ ,
- (c)  $\alpha(fg) = (\alpha f)g = f(\alpha g)$ .

If  $fg = gf$  always, then we say that  $A$  is *commutative*. A Banach space which is also an algebra with a submultiplicative product is a *Banach algebra*.

**Example 3.2.1.** With convolution as a product,  $L^1(\mathbb{R})$  becomes a commutative Banach algebra without identity. Similarly,  $C_0(\mathbb{R})$  is also a commutative Banach algebra without identity (under pointwise products). The space  $\mathcal{B}(X)$  of bounded linear operators on a Banach space  $X$  is also a Banach space under the operator norm, and we have  $\|AB\| \leq \|A\|\|B\|$  with composition as a product. So  $\mathcal{B}(X)$  is a noncommutative Banach algebra, with identity.

### 3.3 Young's Inequality

**Theorem 3.3** (Young's inequality, special case). Fix  $1 \leq p \leq \infty$ . If  $f \in L^p(\mathbb{R})$  and  $g \in L^1(\mathbb{R})$ , then  $f * g \in L^p(\mathbb{R})$  and  $\|f * g\|_p \leq \|f\|_p \|g\|_1$ .

*Proof.* The case  $p = \infty$  is easy by Hölder's inequality and  $p = 1$  is done, so assume  $1 < p < \infty$ . Then

$$|(f * g)(x)| \leq \int |f(y)| |g(x - y)| dy = \int (|f(y)| |g(x - y)|^{1/p}) (|g(x - y)|^{1/p'}) dy,$$

By Hölder's inequality, we can write

$$\begin{aligned}|(f * g)(x)| &\leq \left( \int |f(y)|^p |g(x - y)| dy \right)^{1/p} \left( \int |g(x - y)| dy \right)^{1/p'} \\ &\leq \|g\|_1^{1/p'} \left( \int |f(y)|^p |g(x - y)| dy \right)^{1/p}.\end{aligned}$$

Now taking  $L^p$ -norms, we get

$$\|f * g\|_p^p = \int |(f * g)(x)|^p dx \leq \|g\|_1^{p/p'} \iint |f(y)|^p |g(x - y)| dy dx.$$

By Tonelli's theorem, we can exchange orders and write

$$\|f * g\|_p^p \leq \|g\|_1^{p/p'} \int |f(y)|^p \left( \int |g(x - y)| dx \right) dy \leq \|g\|_1^{1+p/p'} \|f\|_p^p = \|g\|_1^p \|f\|_p^p,$$

so we get the desired inequality  $\|f * g\|_p \leq \|f\|_p \|g\|_1$  after taking  $p$ th roots.  $\square$

**Exercise 3.2** (Young's inequality, general case). Let  $1 \leq p, q, r \leq \infty$  satisfy  $1/r = 1/p + 1/q - 1$ . If  $f \in L^p(\mathbb{R})$  and  $g \in L^q(\mathbb{R})$ , then

$$\|f * g\|_r \leq \|f\|_p \|g\|_q.$$

**Remark.** Recall *Minkowski's inequality* (the triangle inequality in  $L^p(\mathbb{R})$ ):

$$\left\| \sum f_k \right\|_p \leq \sum \|f_k\|_p.$$

*Minkowski's integral inequality* then says that for  $1 \leq p \leq \infty$ ,

$$\left\| \int f_x dx \right\|_p = \left( \int \left| \int f(x, y) dx \right|^p dy \right)^{1/p} \leq \int \left( \int |f(x, y)|^p dy \right)^{1/p} dx = \int \|f_x\|_p dx.$$

One can also use this to prove Young's inequality.

**Remark.** The *Babenko-Beckner constant* is the optimal constant in front of Hölder's inequality:

$$A_p = \left( \frac{p^{1/p}}{(p')^{1/p'}} \right)^{1/2}.$$

The optimal constant in Young's inequality is  $A_p A_q A_{r'}$ , i.e. we have

$$\|f * g\|_r \leq (A_p A_q A_{r'}) \|f\|_p \|g\|_q.$$

### 3.4 The Dirac Delta

**Remark.** Is there an identity for convolution? Suppose there was a function  $\delta \in L^1(\mathbb{R})$  (the *Dirac delta function*) such that  $f * \delta = f$  for all  $f \in L^1(\mathbb{R})$ . Then we have  $(f * \delta)^\wedge = \widehat{f}$ , so

$$\widehat{f}(\xi) \widehat{\delta}(\xi) = \widehat{f}(\xi) \quad \text{for all } f \in L^1(\mathbb{R}).$$

Take  $f(x) = e^{-x^2}$  with  $\widehat{f}(\xi) = e^{-\xi^2}$  and note that  $\widehat{f}(\xi)$  is everywhere nonzero. Then  $\widehat{\delta}(\xi) = 1$  for all  $\xi \in \mathbb{R}$ , which contradicts the Riemann-Lebesgue lemma.

The correct way to work with the Dirac delta is to use the measure

$$\delta(E) = \begin{cases} 1, & 0 \in E, \\ 0, & 0 \notin E. \end{cases}$$

One can then integrate against the measure  $\delta$  to achieve a similar effect.

# Lecture 4

Aug. 28 — Convolution, Part 2

# Lecture 5

## Sept. 2 — Smoothness and Decay

### 5.1 Smoothness and Decay

**Theorem 5.1** (Decay in time implies smoothness in frequency). Assume  $f \in L^1(\mathbb{R})$  and  $x^m f(x) \in L^1(\mathbb{R})$ , where  $m > 0$ . Then

$$\widehat{f} \in C_0^m(\mathbb{R}) = \{g : g, g', \dots, g^{(m)} \in C_0(\mathbb{R})\}.$$

Furthermore, we have

$$\widehat{f}^{(k)} = \frac{d^k}{d\xi^k} \widehat{f} = ((-2\pi i x)^k f(x))^\wedge.$$

*Proof.* The proof is by induction on  $m$ . When  $m = 1$ , we can formally write

$$\begin{aligned} \frac{d}{d\xi} \widehat{f}(\xi) &= \frac{d}{d\xi} \int f(x) e^{-2\pi i \xi x} dx \\ &\stackrel{(*)}{=} \int f(x) \frac{d}{d\xi} e^{-2\pi i \xi x} dx = \int f(x) (-2\pi i x) e^{-2\pi i \xi x} dx = (-2\pi i x f(x))^\wedge(\xi). \end{aligned}$$

It suffices to justify step (\*), which we will do by appealing to the dominated convergence theorem. We can write

$$\widehat{f}'(\xi) = \lim_{\eta \rightarrow 0} \frac{\widehat{f}(\xi + \eta) - \widehat{f}(\xi)}{\eta} = \lim_{\eta \rightarrow 0} \int f(x) \frac{e^{-2\pi i (\xi + \eta)x} - e^{-2\pi i \xi x}}{\eta} dx.$$

Note that we have the pointwise limit

$$f(x) \frac{e^{-2\pi i (\xi + \eta)x} - e^{-2\pi i \xi x}}{\eta} \xrightarrow{\eta \rightarrow 0} f(x) \frac{d}{d\xi} e^{-2\pi i \xi x} = -2\pi i x f(x) e^{-2\pi i \xi x}.$$

Also note that we can bound

$$\left| f(x) \frac{e^{-2\pi i (\xi + \eta)x} - e^{-2\pi i \xi x}}{\eta} \right| = \left| f(x) \frac{e^{-2\pi i \eta x} - 1}{\eta} \right| \leq \left| f(x) \frac{-2\pi i \eta x}{\eta} \right| = |2\pi x f(x)|,$$

where we noted that  $|e^{i\theta} - 1| \leq |\theta|$  for  $\theta \in \mathbb{R}$ . Thus  $2\pi x f(x)$  dominates the integrand and is integrable since  $x f(x) \in L^1(\mathbb{R})$  by assumption, we can conclude (\*) by the dominated convergence theorem. Then  $\widehat{f}' \in C_0(\mathbb{R})$  by the Riemann-Lebesgue lemma, since  $\widehat{f}' = (-2\pi i x f(x))^\wedge$  where  $-2\pi i x f(x) \in L^1(\mathbb{R})$ .

The inductive step is part of Homework 1. □

**Remark.** Recall the position and momentum operators  $Pf(x) = xf(x)$  and  $Mf(x) = f'(x)/2\pi i$ . If  $f, Pf \in L^1(\mathbb{R})$ , then the above theorem tells us that  $(Pf)^\wedge = -M\widehat{f}$ .

## 5.2 Absolute Continuity

**Definition 5.1.** A function  $f : [a, b] \rightarrow \mathbb{C}$  is *absolutely continuous* if for all  $\epsilon > 0$ , there exists  $\delta > 0$  such that if  $\{[a_j, b_j]\}_j$  are countably many non-overlapping intervals, then

$$\sum_j (b_j - a_j) < \delta \quad \text{implies} \quad \sum_j |f(b_j) - f(a_j)| < \epsilon.$$

Define  $\text{AC}_{\text{loc}}(\mathbb{R}) = \{f \in C(\mathbb{R}) : f \text{ is absolutely continuous on every interval } [a, b]\}$ .

**Theorem 5.2** (Fundamental theorem of calculus). *If  $g : [a, b] \rightarrow \mathbb{C}$ , then the following are equivalent:*

1.  $g \in \text{AC}[a, b]$ ;
2. there exists  $f \in L^1[a, b]$  such that for all  $x \in [a, b]$ ,

$$g(x) - g(a) = \int_a^x f(t) dt;$$

3.  $g$  is differentiable at a.e. point,  $g' \in L^1[a, b]$ , and

$$g(x) - g(a) = \int_a^x g'(t) dt.$$

**Remark.** The Cantor-Lebesgue function  $\varphi : [0, 1] \rightarrow [0, 1]$  is continuous with  $\varphi' = 0$  a.e., but

$$\int_0^1 \varphi'(x) dx = 0 \neq 1 = \varphi(1) - \varphi(0).$$

**Lemma 5.1** (Growth lemma). *If  $f : [a, b] \rightarrow \mathbb{R}$  is measurable and differentiable at every point in a measurable set  $E \subseteq [a, b]$ , then*

$$|f(E)|_e \leq \int_E |f'|,$$

where  $|f(E)|_e$  denotes the exterior Lebesgue measure of  $f(E)$ .

**Theorem 5.3** (Banach-Zaretsky theorem). *If  $f : [a, b] \rightarrow \mathbb{R}$ , then the following are equivalent:*

1.  $f \in \text{AC}[a, b]$ ;
2.  $f$  is continuous,  $f$  has bounded variation, and  $|A| = 0$  implies  $|f(A)| = 0$ ;
3.  $f$  is continuous and differentiable a.e.,  $f' \in L^1[a, b]$ , and  $|A| = 0$  implies  $|f(A)| = 0$ .

**Theorem 5.4.** *If  $f : [a, b] \rightarrow \mathbb{C}$  is differentiable on  $[a, b]$  and  $f' \in L^1[a, b]$ , then  $f \in \text{AC}[a, b]$ .*

*Proof.* By the Banach-Zaretsky theorem, it suffices to show that  $|A| = 0$  implies  $|f(A)| = 0$ . If  $|A| = 0$ , then by the growth lemma,

$$|f(A)| \leq \int_A |f'| = 0,$$

which completes the proof. (Technically we should split  $f$  into its real and imaginary parts.) □

### 5.3 Smoothness and Decay, Continued

**Theorem 5.5** (Smoothness in time implies decay in frequency). *If  $f \in L^1(\mathbb{R})$  is everywhere  $m$ -times differentiable and  $f, f', \dots, f^{(m)} \in L^1(\mathbb{R})$ , then*

$$\widehat{f^{(k)}}(\xi) = (2\pi i \xi)^k \widehat{f}(\xi), \quad \text{for } k = 0, \dots, m,$$

hence  $|\widehat{f}(\xi)| \leq |2\pi \xi|^{-k} |\widehat{f^{(k)}}(\xi)| \leq |2\pi \xi|^{-k} \|\widehat{f^{(k)}}\|_\infty \leq |2\pi \xi|^{-k} \|f^{(k)}\|_1$  for  $k = 0, \dots, m$ .

*Proof.* We prove only the case  $m = 1$ , the rest follows by induction. Assume  $f, f' \in L^1(\mathbb{R})$ . By Theorem 5.4, we have  $f \in \text{AC}_{\text{loc}}(\mathbb{R})$ . Hence by the fundamental theorem of calculus,

$$f(x) - f(0) = \int_0^x f'(t) dt.$$

Because  $f'$  is integrable, we get that

$$\lim_{x \rightarrow \infty} f(x) = f(0) + \lim_{x \rightarrow \infty} \int_0^x f'(t) dt = f(0) + \int_0^\infty f'(t) dt.$$

Since  $f$  is integrable and this limit exists, the limit must be 0. Hence  $f \in C_0(\mathbb{R})$ . We can compute

$$\widehat{f'}(\xi) = \int_{-\infty}^\infty f'(x) e^{-2\pi i \xi x} dx = \lim_{\substack{b \rightarrow \infty \\ a \rightarrow -\infty}} \int_a^b f'(x) e^{-2\pi i \xi x} dx.$$

Since  $f$  is absolutely continuous, we can integrate by parts to get

$$\widehat{f'}(\xi) = \lim_{\substack{b \rightarrow \infty \\ a \rightarrow -\infty}} \left[ f(b) e^{-2\pi i \xi b} - f(a) e^{-2\pi i \xi a} + (2\pi i \xi) \int_a^b f(x) e^{-2\pi i \xi x} dx \right] = (2\pi i \xi) \widehat{f}(\xi),$$

which proves the desired result. □

**Remark.** Note that for the absolute continuity arguments, we need to first restrict to a finite interval and then take limits, since we only know that  $f \in \text{AC}_{\text{loc}}(\mathbb{R})$ .

### 5.4 Approximate Identities

**Remark.** Recall that if we take  $g_T = \chi_{[-T, T]}/2T$ , then we have  $(f * g_T)(x) = \text{Avg}_{[x-T, x+T]} f$ . As  $T \rightarrow 0$ , this converges to  $f$  if  $f$  is continuous, and converges a.e. to  $f$  if  $f$  is integrable. In particular, this is almost like a identity for the convolution operation.

**Definition 5.2.** If  $k_\lambda \in L^1(\mathbb{R})$  for  $\lambda > 0$  (or sometimes  $\lambda \in \mathbb{N}$ ) satisfy:

- (a) Normalization:  $\int_{-\infty}^\infty k_\lambda = 1$  for every  $\lambda$ ,
- (b)  $L^1$ -boundedness:  $\sup_\lambda \|k_\lambda\|_1 = \sup_\lambda \int_{-\infty}^\infty |k_\lambda| < \infty$ ,
- (c)  $L^1$ -concentration:  $\lim_{\lambda \rightarrow \infty} \int_{|x| \geq \delta} |k_\lambda| = 0$  for every  $\delta > 0$ ,

then we say that  $\{k_\lambda\}$  is an *approximate identity (for convolution)*.

**Exercise 5.1.** If  $k \in L^1(\mathbb{R})$  and  $\int_{-\infty}^{\infty} k = 1$ , then  $k_\lambda(x) = \lambda k(\lambda x)$  forms an approximate identity.

**Remark.** If we choose  $k_\lambda$  to be nice, then  $f * k_\lambda$  will also be nice and “close” to  $f$ .



# Lecture 6

## Sept. 4 — Approximate Identities

### 6.1 Properties of Approximate Identities

**Theorem 6.1.** *If  $\{k_\lambda\}$  is an approximate identity, then for all  $f \in L^1(\mathbb{R})$ ,*

$$\lim_{\lambda \rightarrow \infty} \|f * k_\lambda - f\|_1 = 0.$$

*That is,  $f * k_\lambda \rightarrow f$  in  $L^1$ -norm.*

*Proof.* We have already seen that  $f * k_\lambda \in L^1(\mathbb{R})$ . Then

$$\|f - f * k_\lambda\|_1 = \int |f(x) - (f * k_\lambda)(x)| dx = \int \left| f(x) \int k_\lambda(t) dt - \int f(x-t) k_\lambda(t) dt \right| dx,$$

where we used that  $\int k_\lambda(t) dt = 1$ . Collecting terms and taking absolute values inside,

$$\|f - f * k_\lambda\|_1 \leq \iint |f(x) - f(x-t)| |k_\lambda(t)| dt dx.$$

By Tonelli's theorem, we can exchange orders to get

$$\|f - f * k_\lambda\|_1 \leq \int |k_\lambda(t)| \left( \int |f(x) - T_t f(x)| dx \right) dt = \int |k_\lambda(t)| \|f - T_t f\|_1 dt.$$

We split this integral into two parts:

$$\|f - f * k_\lambda\|_1 \leq \int_{|t| < \delta} |k_\lambda(t)| \|f - T_t f\|_1 dt + \int_{|t| \geq \delta} |k_\lambda(t)| \|f - T_t f\|_1 dt.$$

By the strong continuity of translation, we know that  $\lim_{t \rightarrow 0} \|f - T_t f\|_1 = 0$ , so for any  $\epsilon > 0$ , there exists  $\delta > 0$  such that  $|t| < \delta$  implies  $\|f - T_t f\|_1 < \epsilon$ . This lets us estimate the first integral:

$$\|f - f * k_\lambda\|_1 \leq \epsilon \int_{|t| < \delta} |k_\lambda(t)| dt + \int_{|t| \geq \delta} |k_\lambda(t)| \|f - T_t f\|_1 dt.$$

For the second integral, we can use  $\|f - T_t f\|_1 \leq \|f\|_1 + \|T_t f\|_1 = 2\|f\|_1$  to get

$$\|f - f * k_\lambda\|_1 \leq \epsilon \int_{|t| < \delta} |k_\lambda(t)| dt + 2\|f\|_1 \int_{|t| \geq \delta} |k_\lambda(t)| dt \leq \epsilon K + 2\|f\|_1 \epsilon$$

where  $K = \sup_\lambda \|k_\lambda\|_1 < \infty$  and  $\lambda$  is large enough (as  $\int_{|t| \geq \delta} |k_\lambda(t)| dt \rightarrow 0$ ). So  $\|f - f * k_\lambda\|_1 \rightarrow 0$ .  $\square$

**Exercise 6.1.** Show that for  $1 \leq p < \infty$ , we still have  $\|f - f * k_\lambda\|_p \rightarrow 0$  as  $\lambda \rightarrow \infty$  for  $f \in L^p(\mathbb{R})$ . For  $p = \infty$ , show that if  $f \in C_0(\mathbb{R})$ , then  $\|f - f * k_\lambda\|_\infty \rightarrow 0$  as  $\lambda \rightarrow \infty$ , that is  $f * k_\lambda \rightarrow f$  uniformly.

**Exercise 6.2.** Show that if  $f \in C_b(\mathbb{R})$ , then for every compact set  $K \subseteq \mathbb{R}$ ,

$$\lim_{\lambda \rightarrow \infty} \|(f - f * k_\lambda)\chi_K\|_\infty = 0.$$

**Definition 6.1.** A function  $f$  is *Hölder continuous* with exponent  $\alpha > 0$  if

$$|f(x) - f(y)| \leq K|x - y|^\alpha$$

for some constant  $K$  and all  $x, y$ . If  $\alpha = 1$ , then we say that  $f$  is *Lipschitz*.

**Remark.** If  $f$  is Hölder continuous with exponent  $\alpha > 1$ , then the mean value theorem implies that  $f$  is constant. Thus the interesting range for Hölder continuity is  $0 < \alpha \leq 1$ .

**Exercise 6.3.** Let  $f$  be bounded and Hölder continuous with exponent  $0 < \alpha \leq 1$ , then show that

$$f * k_\lambda \rightarrow f \quad \text{uniformly on } \mathbb{R}.$$

**Remark.** If  $f$  is differentiable and  $f'$  is bounded, then  $f$  is Lipschitz.

**Remark.** Recall the *Lebesgue differentiation theorem*, which says that if  $f \in L^1_{\text{loc}}(\mathbb{R})$ , then

$$(f * g_T)(x) = \frac{1}{2T} \int_{x-T}^{x+T} f(t) dt \longrightarrow f(x) \quad \text{for a.e. } x.$$

where  $g_T = \chi_{[-T, T]}/(2T)$ . The points where the limit holds are called the *Lebesgue points* of  $f$ .

**Theorem 6.2.** Assume  $k$  is bounded and compactly supported and  $\int k = 1$ . Set  $k_\lambda(x) = \lambda k(\lambda x)$  for  $\lambda > 0$ . Then for any  $f \in L^1(\mathbb{R})$ ,

$$f * k_\lambda \rightarrow f \quad \text{pointwise a.e.}$$

Moreover, the pointwise limit holds at every Lebesgue point of  $f$ .

*Proof.* Assume  $\text{supp}(k) \subseteq [-R, R]$ . We can write

$$\begin{aligned} \lim_{\lambda \rightarrow \infty} |f(x) - (f * k_\lambda)(x)| &= \lim_{\lambda \rightarrow \infty} \left| f(x) \int k_\lambda(x - t) dt - \int f(x) k_\lambda(x - t) dt \right| \\ &\leq \lim_{\lambda \rightarrow \infty} \int |f(x) - f(t)| \lambda |k(\lambda x - \lambda t)| dt \\ &\leq \lim_{\lambda \rightarrow \infty} \lambda \int_{x-R/\lambda}^{x+R/\lambda} |f(x) - f(t)| |k(\lambda x - \lambda t)| dt. \end{aligned}$$

Making a change of variables  $T = R/\lambda$ , we have

$$\lim_{\lambda \rightarrow \infty} |f(x) - (f * k_\lambda)(x)| \leq \lim_{T \rightarrow 0} \frac{1}{2T} \int_{x-T}^{x+T} |f(x) - f(t)| dt \cdot \|k\|_\infty = 0$$

for every Lebesgue point  $x$  by the Lebesgue differentiation theorem. □

## 6.2 Density Results and Smooth Urysohn Lemma

**Theorem 6.3.**  $C_c^m(\mathbb{R})$  is dense in  $L^p(\mathbb{R})$  for  $m > 0$  and  $1 \leq p < \infty$ .

*Proof.* Fix  $\epsilon > 0$ . Choose  $k \in C_c^m(\mathbb{R})$  with  $\int k = 1$ , and set  $k_\lambda(x) = \lambda k(\lambda x)$ . Note that there exists a compactly supported  $g \in L^p(\mathbb{R})$  with  $\|f - g\|_p < \epsilon$  (e.g. take  $g = f\chi_{[-R,R]}$  for large enough  $R$ , this works since  $f\chi_{[-R,R]}$  converges pointwise to  $f$  as  $R \rightarrow \infty$  and is dominated by  $f$ , so the dominated convergence theorem implies that  $f\chi_{[-R,R]} \rightarrow f$  in  $L^p$ -norm). Then note that  $g * k_\lambda \in C_c^m(\mathbb{R})$  and  $g * k_\lambda \rightarrow g$  in  $L^p$ -norm, so there exists  $\lambda$  such that  $\|g - g * k_\lambda\|_p < \epsilon$ . Thus

$$\|f - g * k_\lambda\|_p \leq \|f - g\|_p + \|g - g * k_\lambda\|_p < 2\epsilon$$

which implies the desired result.  $\square$

**Corollary 6.3.1.**  $C_c^\infty(\mathbb{R})$  is dense in  $L^p(\mathbb{R})$  for  $1 \leq p < \infty$ .

**Remark.** The above proof would work for  $m = 0$  but becomes circular: The step  $g * k_\lambda \in C_c^m(\mathbb{R})$  relies on the strong continuity of translation, which we proved by first showing it for  $C_c(\mathbb{R})$  and then by an extension by density to  $L^p(\mathbb{R})$ . In particular, we needed to already know that  $C_c(\mathbb{R})$  is dense in  $L^p(\mathbb{R})$ .

**Proposition 6.1** ( $C^\infty$  Urysohn's lemma). *If  $K \subseteq \mathbb{R}$  is compact and  $U \subseteq K$  is open, then there exists  $f \in C_c^\infty(\mathbb{R})$  such that  $0 \leq f \leq 1$ ,  $f = 1$  on  $K$ , and  $f = 0$  on  $U^c$ .*

*Proof.* Since  $K$  is compact and  $U^c$  is closed, we have

$$d = \text{dist}(K, U^c) = \inf\{|x - y| : k \in K, y \notin U\} > 0.$$

Set  $V = \{y \in \mathbb{R} : \text{dist}(y, K) < d/3\}$ , and choose any  $k \in C_c^\infty(\mathbb{R})$  such that  $\text{supp}(k) \subseteq [-d/3, d/3]$  and  $\int k = 1$ . Take  $f = k * \chi_V \in C_c^\infty(\mathbb{R})$ , which has  $\text{supp}(f) \subseteq \text{supp}(k) + V \subseteq U$ . If  $x \in K$ , then

$$f(x) = \int_V k(x - y) dy = \int k = 1.$$

One can check that  $0 \leq f \leq 1$  and  $f = 0$  on  $U^c$  as an exercise, which would prove the result.  $\square$

# Lecture 7

Sept. 18 —

# Lecture 8

Sept. 23 —

# Lecture 9

## Sept. 25 — Kernels and Schwartz Space

### 9.1 More Kernels

**Remark.** Recall that if  $\{k_\lambda\}$  (where  $k_\lambda(x) = \lambda k(\lambda x)$ ) is an approximate identity, then  $f * k_\lambda \rightarrow f$  in  $L^p$ -norm. We also have

$$(f * k_\lambda)^\wedge = \widehat{f} \cdot \widehat{k}_\lambda.$$

Note that  $\widehat{k}_\lambda(\xi) = \widehat{k}(\xi/\lambda)$ , so  $\widehat{k}_\lambda(\xi) \rightarrow 1$  pointwise. If the Dirichlet kernel  $d_{2\pi\lambda}(\xi) = \sin(2\pi\lambda\xi)/(\pi\xi)$  were integrable, then we would have  $\widehat{d_{2\pi\lambda}}(\xi) = \chi_{[-\lambda, \lambda]}(\xi)$ , so we must have  $d_{2\pi\lambda} \notin L^1(\mathbb{R})$ .

Some alternatives are the following:

1. The Fejér kernel  $w_\lambda(\xi) = d_{2\pi\lambda}^2(\xi) \in L^1(\mathbb{R})$ . We saw this in the proof of the inversion formula.
2. The *de la Vallée Poussin kernel*  $v_\lambda$ , which has  $\widehat{v}_\lambda$  as a trapezoid which is 1 on  $[-\lambda, \lambda]$  and decays linearly to 0 on  $[-2\lambda, -\lambda]$  and  $[\lambda, 2\lambda]$ . One has

$$(f * v_\lambda)^\wedge = \widehat{f} \cdot \widehat{v}_\lambda = \widehat{f} \quad \text{on } [-\lambda, \lambda].$$

Explicitly, one can define  $v(x) = 2w_2(x) - w(x)$  and  $v_\lambda(x) = \lambda v(\lambda x)$ .

3. The *Poisson kernel*  $p(x) = 1/\pi(x^2 + 1)$ .
4. The *Gauss kernel*  $\phi(x) = e^{-\pi x^2}$ .

**Exercise 9.1.** Show that if  $f \in L^1(\mathbb{R})$ , then  $\text{supp}(\widehat{f})$  is compact if and only if  $f = f * g$  for some  $g \in L^1(\mathbb{R})$ . Hint: Use the de la Vallée Poussin kernel.

**Exercise 9.2.** Let  $\Phi = \widehat{\phi}$ , where  $\phi$  is the Gauss kernel. Show that  $\Phi'(\xi) = -2\pi\xi\Phi(\xi)$ . Then solve this differential equation to get  $\Phi(\xi) = \Phi(0)\phi(\xi)$ . Finally show that  $\Phi(0) = 1$ , and conclude  $\Phi(\xi) = \phi(\xi)$ .

**Remark.** There are other ways to find functions which are their own Fourier transforms. The inversion formula says that if  $f, \widehat{f} \in L^1(\mathbb{R})$ , then we have

$$f(x) = (\widehat{f})^\vee(x) = f^{\wedge\wedge}(-x) = f^{\wedge\wedge\wedge\wedge}(x).$$

In particular, for  $f$  sufficiently nice, if we take  $g = f + f^\wedge + f^{\wedge\wedge} + f^{\wedge\wedge\wedge}$ , then  $\widehat{g} = g$ .

**Theorem 9.1** (Weierstrass approximation theorem). *If  $f \in C[a, b]$  and  $\epsilon > 0$ , then there exists a polynomial  $p$  such that  $\|f - p\|_\infty = \sup_{x \in [a, b]} |f(x) - p(x)| < \epsilon$ .*

*Proof.* Fix  $f \in C[a, b]$ , and choose  $[a, b] \subseteq (-R, R)$ . Extend  $f$  to a function  $g \in C_0(\mathbb{R})$  on  $\mathbb{R}$  which equals  $f$  on  $[a, b]$  and is supported in  $(-R, R)$ . Let  $\phi$  be the Gauss kernel, and choose  $\lambda$  so that

$$\|g - g * \phi_\lambda\|_\infty < \frac{\epsilon}{2}.$$

Note that  $\phi_\lambda(x) = \lambda e^{-\pi\lambda^2 x^2}$  is analytic and has a Taylor expansion

$$\phi_\lambda(x) = \sum_{n=0}^{\infty} \lambda \frac{(-\pi\lambda^2 x^2)^n}{n!} = \sum_{n=0}^{\infty} \frac{(-1)^n \pi^n \lambda^{2n+1}}{n!} x^{2n}.$$

Set  $q(x) = \sum_{n=0}^N \frac{(-1)^n \pi^n \lambda^{2n+1}}{n!} x^{2n}$ . If  $N$  is large enough, then we will have

$$\sup_{|x| \leq 2R} |\phi_\lambda(x) - q(x)| < \frac{\epsilon}{2\|g\|_1}$$

since the Taylor series converges uniformly on compact sets. Then

$$|(g * \phi_\lambda)(x) - (g * q)(x)| \leq \int_{-R}^R |g(y)| |\phi_\lambda(x - y) - q(x - y)| dy \leq \frac{\epsilon}{2\|g\|_1} \int_{-R}^R |g(y)| dy < \frac{\epsilon}{2}$$

for  $|x| \leq R$ . So  $|f(x) - (g * q)(x)| \leq \epsilon$  for  $x \in [a, b]$ . Finally, observe that

$$(g * q)(x) = \sum_{n=0}^N \frac{(-1)^n \pi^n \lambda^{2n+1}}{n!} \int g(y) (x - y)^{2n} dy,$$

which is a polynomial by the binomial theorem. So we can take  $p = g * q$ . □

## 9.2 Schwartz Space

**Definition 9.1.** Define the *Schwartz space*  $\mathcal{S}(\mathbb{R})$  to be

$$\mathcal{S}(\mathbb{R}) = \{f \in C^\infty(\mathbb{R}) : x^m f^{(n)}(x) \in L^\infty(\mathbb{R}) \text{ for all } m, n \geq 0\}.$$

**Remark.** Note that  $|x^m f^{(n)}(x)| \leq C_{m,n}$  for some constant  $C_{m,n}$ , so

$$|f^{(n)}(x)| \leq \frac{C_{m,n}}{|x|^m}.$$

In particular, for every  $n$  and polynomial  $p$ , there exists a constant  $C_{n,p}$  such that

$$|f^{(n)}(x)| \leq \frac{C_{n,p}}{|p(x)|}.$$

Note, however, that this does not imply  $f$  has exponential decay.

**Remark.** Note that  $\rho_{m,n}(f) = \|x^m f^{(n)}\|_\infty$  defines a *seminorm* for each  $m, n \geq 0$ , but not a norm.<sup>1</sup>

<sup>1</sup>Recall that a *seminorm*  $\rho$  is a function satisfying  $0 \leq \rho(f) < \infty$ ,  $\rho(cf) = |c|\rho(f)$ , and  $\rho(f + g) \leq \rho(f) + \rho(g)$ . If we additionally have  $\rho(f) = 0$  if and only if  $f = 0$ , then  $\rho$  is a *norm*.

**Remark.** Let  $f \in \mathcal{S}(\mathbb{R})$ . Then

$$\begin{aligned} \|x^m f^{(n)}\|_1 &= \int_{|x| \leq 1} |x^m f^{(n)}(x)| dx + \int_{|x| \geq 1} |x^m f^{(n)}(x)| dx \\ &\leq 2\|x^m f^{(n)}\|_\infty + \int_{|x| \geq 1} \frac{|x^{m+2} f^{(n)}(x)|}{|x|^2} dx \leq 2\|x^m f^{(n)}\|_\infty + C\|x^{m+2} f^{(n)}\|_\infty. \end{aligned}$$

In particular, if the  $L^\infty$ -norms are controlled, then so are the  $L^1$ -norms.

**Exercise 9.3.** Recall the smoothness and decay theorems: The Fourier transform interchanges smoothness and decay. Write  $Df = f'$ , and show that

$$(D^n((-2\pi i x)^m f(x)))^\wedge(\xi) = (2\pi i \xi)^n D^m \hat{f}(\xi).$$

Note that we have

$$D^n((-2\pi i x)^m f(x)) = \sum_{j=0}^n \binom{n}{j} D^j (-2\pi i x)^m f^{(n-j)}(x),$$

so in particular, the Schwartz condition on  $f$  implies the Schwartz condition on  $\hat{f}$ .

**Theorem 9.2.** If  $f \in \mathcal{S}(\mathbb{R})$ , then  $\hat{f} \in \mathcal{S}(\mathbb{R})$ . Moreover, we have  $f = (\hat{f})^\vee$  by the inversion formula, so the Fourier transform  $\mathcal{F} : \mathcal{S}(\mathbb{R}) \rightarrow \mathcal{S}(\mathbb{R})$  by  $f \mapsto \hat{f}$  is a bijection.

**Remark.** Note that  $C_c^\infty(\mathbb{R}) \subsetneq \mathcal{S}(\mathbb{R})$ , and we will see later that  $\mathcal{F}(C_c^\infty(\mathbb{R})) \subseteq \mathcal{S}(\mathbb{R}) \setminus C_c^\infty(\mathbb{R})$ .